lib/FStar.Set.fst
@@ -21,20 +21,20 @@ module FStar.Set
 #set-options "--initial_fuel 0 --max_fuel 0 --initial_ifuel 0 --max_ifuel 0"
 open FStar.FunctionalExtensionality
 
-(* abstract *) type set a = a -> Tot bool
-(* abstract *) type Equal (#a:Type) (s1:set a) (s2:set a) = FEq s1 s2
+abstract type set a = a -> Tot bool
+abstract type Equal (#a:Type) (s1:set a) (s2:set a) = FEq s1 s2
 
 (* destructors *)
 
-(* abstract *) val mem : 'a -> set 'a -> Tot bool
+abstract val mem : 'a -> set 'a -> Tot bool
 let mem x s = s x
 
 (* constructors *)
-(* abstract *) val empty      : #a:Type -> Tot (set a)
-(* abstract *) val singleton  : 'a -> Tot (set 'a)
-(* abstract *) val union      : set 'a -> set 'a -> Tot (set 'a)
-(* abstract *) val intersect  : set 'a -> set 'a -> Tot (set 'a)
-(* abstract *) val complement : set 'a -> Tot (set 'a)
+abstract val empty      : #a:Type -> Tot (set a)
+abstract val singleton  : 'a -> Tot (set 'a)
+abstract val union      : set 'a -> set 'a -> Tot (set 'a)
+abstract val intersect  : set 'a -> set 'a -> Tot (set 'a)
+abstract val complement : set 'a -> Tot (set 'a)
 
 
 let empty           = fun #a x -> false
@@ -44,41 +44,41 @@ let intersect s1 s2 = fun x -> s1 x && s2 x
 let complement s    = fun x -> not (s x)
 
 (* ops *)
-(* abstract *) val subset       : set 'a -> set 'a -> Tot bool
+abstract val subset       : set 'a -> set 'a -> Tot bool
 let subset s1 s2 = (intersect s1 s2) = s1
 
 (* Properties *)
-(* abstract *) val mem_empty: #a:Type -> x:a -> Lemma
+abstract val mem_empty: #a:Type -> x:a -> Lemma
    (requires True)
    (ensures (not (mem x empty)))
    [SMTPat (mem x empty)]
 
-(* abstract *) val mem_singleton: #a:Type -> x:a -> y:a -> Lemma
+abstract val mem_singleton: #a:Type -> x:a -> y:a -> Lemma
    (requires True)
    (ensures (mem y (singleton x) = (x=y)))
    [SMTPat (mem y (singleton x))]
 
-(* abstract *) val mem_union: #a:Type -> x:a -> s1:set a -> s2:set a -> Lemma
+abstract val mem_union: #a:Type -> x:a -> s1:set a -> s2:set a -> Lemma
    (requires True)
    (ensures (mem x (union s1 s2) = (mem x s1 || mem x s2)))
    [SMTPat (mem x (union s1 s2))]
 
-(* abstract *) val mem_intersect: #a:Type -> x:a -> s1:set a -> s2:set a -> Lemma
+abstract val mem_intersect: #a:Type -> x:a -> s1:set a -> s2:set a -> Lemma
    (requires True)
    (ensures (mem x (intersect s1 s2) = (mem x s1 && mem x s2)))
    [SMTPat (mem x (intersect s1 s2))]
 
-(* abstract *) val mem_complement: #a:Type -> x:a -> s:set a -> Lemma
+abstract val mem_complement: #a:Type -> x:a -> s:set a -> Lemma
    (requires True)
    (ensures (mem x (complement s) = not(mem x s)))
    [SMTPat (mem x (complement s))]
 
-(* abstract *) val mem_subset: #a:Type -> s1:set a -> s2:set a -> Lemma
+abstract val mem_subset: #a:Type -> s1:set a -> s2:set a -> Lemma
    (requires (forall x. mem x s1 ==> mem x s2))
    (ensures (subset s1 s2))
    [SMTPat (subset s1 s2)]
 
-(* abstract *) val subset_mem: #a:Type -> s1:set a -> s2:set a -> Lemma
+abstract val subset_mem: #a:Type -> s1:set a -> s2:set a -> Lemma
    (requires (subset s1 s2))
    (ensures (forall x. mem x s1 ==> mem x s2))
    [SMTPat (subset s1 s2)]
@@ -93,17 +93,17 @@ let mem_subset     #a s1 s2   = cut (Equal (intersect s1 s2) s1)
 
 (* extensionality *)
 
-(* abstract *) val lemma_equal_intro: #a:Type -> s1:set a -> s2:set a -> Lemma
+abstract val lemma_equal_intro: #a:Type -> s1:set a -> s2:set a -> Lemma
     (requires  (forall x. mem x s1 = mem x s2))
     (ensures (Equal s1 s2))
     [SMTPatT (Equal s1 s2)]
 
-(* abstract *) val lemma_equal_elim: #a:Type -> s1:set a -> s2:set a -> Lemma
+abstract val lemma_equal_elim: #a:Type -> s1:set a -> s2:set a -> Lemma
     (requires (Equal s1 s2))
     (ensures  (s1 = s2))
     [SMTPatT (Equal s1 s2)]
 
-(* abstract *) val lemma_equal_refl: #a:Type -> s1:set a -> s2:set a -> Lemma 
+abstract val lemma_equal_refl: #a:Type -> s1:set a -> s2:set a -> Lemma 
     (requires (s1 = s2))
     (ensures  (Equal s1 s2))
     [SMTPatT (Equal s1 s2)]
