lib/FStar.Heap.fst
@@ -6,7 +6,7 @@ module FStar.Heap
 #set-options "--initial_fuel 0 --max_fuel 0 --initial_ifuel 1 --max_ifuel 1"
 open FStar.Set
 assume new type heap : Type0
-(* abstract *) type ref (a:Type) = 
+abstract type ref (a:Type) = 
   | MkRef of a //this implementation of ref is not realistic; it's just to get the universes right
 type aref =
   | Ref : #a:Type -> r:ref a -> aref
