lib/ext.fst
@@ -24,5 +24,3 @@ opaque type FEq (#a:Type) (#b:Type) (f:efun a b) (g:efun a b) =
 
 assume Extensionality : forall (a:Type) (b:Type) (f: efun a b) (g: efun a b).
                         {:pattern FEq #a #b f g} FEq #a #b f g <==> f=g
-
-end
